Move to generic hash_tree_root.

src/dafny/beacon/StateTransition.dfy
@@ -48,13 +48,8 @@ module StateTransition {
      *  
      *  @todo   Use the hash_tree_root from Merkle.
      */
-    function method hash_tree_root(s: BeaconState) : Bytes32 
-        ensures hash_tree_root(s) != EMPTY_BYTES32
-
-    // function method hash_tree_root_block(s: BeaconBlock) : Bytes32 
-    function method hash_tree_root_block_header(b: BeaconBlockHeader) : Bytes32 
-        ensures hash_tree_root_block_header(b) == EMPTY_BYTES32 <==> isGenesisBlockHeader(b)
-
+    function method hash_tree_root<T>(t : T) : Bytes32 
+        ensures hash_tree_root(t) != EMPTY_BYTES32
     /** 
      * @link{https://notes.ethereum.org/@djrtwo/Bkn3zpwxB?type=view} 
      * The beacon chain’s state (BeaconState) is the core object around 
